Add some GC-related ghost states

src/program_proof/mvcc/mvcc_ghost.v
@@ -1,8 +1,10 @@
 From Perennial.program_proof Require Import disk_prelude.
-From iris.base_logic.lib Require Import ghost_map.
-From iris.algebra Require Import dfrac_agree.
+From iris.algebra Require Import dfrac_agree gset.
+From iris.algebra.lib Require Import mono_nat gmap_view.
 
 Local Definition key_fixedR := gmapR u64 (dfrac_agreeR (leibnizO nat)).
+Local Definition tidsR := gmap_viewR nat (leibnizO unit).
+Local Definition sid_tidsR := gmapR u64 (dfrac_agreeR (leibnizO (gset u64))).
 
 Class mvcc_ghostG Σ :=
   {
@@ -10,11 +12,17 @@ Class mvcc_ghostG Σ :=
     mvcc_ghost_dbmaps :> ghost_mapG Σ (nat * u64) u64;
     mvcc_ghost_key_fixed :> inG Σ key_fixedR;
     *)
-    (* XXX: remove this *)
-    mvcc_ghost_versG :> ghost_varG Σ (list (u64 * u64 * u64))
+    mvcc_active_tidsG :> inG Σ tidsR;
+    mvcc_active_tids_siteG :> inG Σ sid_tidsR;
+    mvcc_min_tidG :> inG Σ mono_natR;
   }.
 
-Definition mvcc_ghostΣ := #[(*ghost_mapΣ (nat * u64) u64; GFunctor key_fixedR;*) (* XXX *) ghost_varΣ (list (u64 * u64 * u64))].
+Definition mvcc_ghostΣ :=
+  #[(*ghost_mapΣ (nat * u64) u64; GFunctor key_fixedR;*)
+     GFunctor tidsR;
+     GFunctor sid_tidsR;
+     GFunctor mono_natR
+   ].
 
 Global Instance subG_mvcc_ghostG {Σ} :
   subG mvcc_ghostΣ Σ → mvcc_ghostG Σ.
@@ -27,7 +35,9 @@ Record mvcc_names :=
     mvcc_fixed : gname;
     *)
     (* XXX *)
-    tuple_vers_gn : gname
+    mvcc_active_tids_gn: gname;
+    mvcc_active_tids_site_gn: gname;
+    mvcc_min_tid_gn : gname
   }.
 
 Section definitions.
@@ -46,19 +56,47 @@ Theorem view_ptsto_agree (k v v' : u64) :
   view_ptsto k v -∗ view_ptsto k v' -∗ ⌜v = v'⌝.
 Admitted.
 
+Definition active_tids_auth γ tids : iProp Σ :=
+  own γ.(mvcc_active_tids_gn) (gmap_view_auth (DfracOwn 1) tids).
+
+Definition active_tid γ (tid : nat) : iProp Σ :=
+  own γ.(mvcc_active_tids_gn) (gmap_view_frag (V:=leibnizO unit) tid (DfracOwn 1) tt).
+
+Definition active_tids_site γ (sid : u64) tids : iProp Σ :=
+  own γ.(mvcc_active_tids_site_gn) {[sid := to_dfrac_agree (DfracOwn (1/2)) tids]}.
+
+Definition min_tid_auth γ tid : iProp Σ :=
+  own γ.(mvcc_min_tid_gn) (●MN tid).
+
+Definition min_tid_lb γ tid : iProp Σ :=
+  own γ.(mvcc_min_tid_gn) (◯MN tid).
+
+Theorem active_ge_min γ tid tidlb :
+  active_tid γ tid -∗
+  min_tid_lb γ tidlb -∗
+  ⌜(tid ≥ tidlb)%nat⌝.
+Admitted.
+
 (*
 Definition fixed_ptsto γ (q : Qp) (key : u64) (fixed : nat) : iProp Σ :=
   own γ.(mvcc_fixed) {[key := to_dfrac_agree (DfracOwn q) (fixed : (leibnizO _))]}.
 
 Definition db_ptsto γ (dq : dfrac) (ts : nat) (key : u64) (val : u64) : iProp Σ :=
   (ts, key) ↪[γ.(mvcc_dbmaps)]{dq} val.
+*)
 
 Definition mvcc_invariant γ : iProp Σ :=
+  ∃ tidmin tidsactive,
+    min_tid_auth γ tidmin ∗
+    active_tids_auth γ tidsactive ∗
+    (* TODO: tidsactive is the union of tids of each *)
+    ⌜∀ tid, tid ∈ (dom (gset nat) tidsactive) -> (tid ≥ tidmin)%nat⌝.
+  (*
   ∃ dbmaps,
     ghost_map_auth γ.(mvcc_dbmaps) 1 dbmaps.
+  *)
 
 Definition mvcc_inv γ : iProp Σ :=
   inv mvccN (mvcc_invariant γ).
-*)
 
 End definitions.
